## Niech $F:A\xrightarrow[\text{1-1}]{\text{na}}B$ będzie [[Bijekcja|bijekcją]]. Wiemy, że 
### (a) $\forall x\in A\:\exists!y\in B: (x,y) \in F$ 
### (b) $\forall y\in B \: \exists! x\in A: (x,y) \in F$
## Rozważmy zatem $G=\{(y,x):(x,y)\in F\}$. $G$ jest:
### (1) *[[Funkcja|Funkcją]]* - z (b).
### (2) [[Iniekcja|Iniekcją]] - z (a).
### (3) [[Suriekcja|Suriekcją]] - z (b).
### (4) *[[Bijekcja|Bijekcją]]* - z (2) i (3).

## Funkcję $G:B\xrightarrow[\text{1-1}]{\text{na}}A$  nazywamy **funkcją odwrotną** $F^{-1}$.
## **Własności**:
### (i) $(F^{-1} \circ F)(x) = F^{-1}(F(x)) = id_{A}$
### (ii) $(F \circ F^{-1})(y) = F(F^{-1}(y))= id_{B}$
